examples/ecommerce/tests/EcommerceFixedGens.v
@@ -93,7 +93,7 @@ Definition gEcommerceFixedAction (env : Env): GOpt Action :=
             backtrack [
                 (1%nat, call purchase.(buyer) 0 (buyer_confirm_delivery purchaseId));
                 (1%nat, let buyer_dispute_delivery_commmitment := hash_bid purchaseId constant_buyer_bit constant_buyer_nonce in
-                        item <- returnGen (FMap.find 2%nat(*purchase.(itemId)*) state.(listings));;
+                        item <- returnGen (FMap.find purchase.(itemId) state.(listings));;
                         call purchase.(buyer) item.(item_value) (buyer_dispute_delivery purchaseId buyer_dispute_delivery_commmitment));
                 (1%nat, call state.(seller) 0 (seller_call_timeout purchaseId))
             ]
@@ -118,75 +118,4 @@ Definition gEcommerceFixedAction (env : Env): GOpt Action :=
     )
   ].
   
-(*
-
-Definition gEcommerceFixedAction (env : Env): GOpt Action :=
-  let call caller amount msg :=
-      returnGenSome {|
-          act_origin := caller;
-          act_from := caller;
-          act_body := act_call contract_addr amount (@serialize EcommerceFixed.Msg EcommerceFixed.Msg_serializable msg)
-      |} in
-  state <- returnGen (get_contract_state EcommerceFixed.State env contract_addr);;
-  let buyer_balance := env.(env_account_balances) purchase_buyer in
-  let itemId := item1_Id%nat in
-  let cur_slot := env.(env_chain).(current_slot) in
-  let buyer_dispute_delivery_commmitment := hash_bid purchaseId true 42%N in
-  match FMap.find itemId state.(listings), cur_slot with
-  | Some _item, 1%nat => (* This is done explicitly with cur_slot to make sure that we know the purchaseId in this generator. *)
-      (* buyer_request_purchase *)
-      call purchase_buyer _item.(item_value) (buyer_request_purchase itemId "notes here")
-  | Some _item, _ =>
-  backtrack[
-    (19%nat,
-      match FMap.find purchaseId state.(purchases) with
-      | Some purchase => 
-          match purchase.(purchase_state) with
-          | requested =>
-                (* buyer_abort || seller_reject_contract || seller_accept_contract *)
-                backtrack [
-                    (1%nat, call purchase.(buyer) 0 (buyer_abort purchaseId));
-                    (1%nat, call state.(seller) 0 (seller_reject_contract purchaseId));
-                    (5%nat, call state.(seller) 0 (seller_accept_contract purchaseId))
-                ]
-          | accepted =>
-                (* buyer_call_timeout || seller_item_was_delivered *)
-                backtrack [
-                    (1%nat, call purchase.(buyer) 0 (buyer_call_timeout purchaseId));
-                    (4%nat, call state.(seller) 0 (seller_item_was_delivered purchaseId))
-                ]
-          | delivered =>
-                (* buyer_confirm_delivery || buyer_dispute_delivery || seller_call_timeout *)
-                backtrack [
-                    (1%nat, call purchase.(buyer) 0 (buyer_confirm_delivery purchaseId));
-                    (1%nat, call purchase.(buyer) _item.(item_value) (buyer_dispute_delivery purchaseId buyer_dispute_delivery_commmitment));
-                    (4%nat, call state.(seller) 0 (seller_call_timeout purchaseId))
-                ]
-          | dispute =>
-                random_bit <- bindGen (oneOf[returnGen true; returnGen false]) returnGenSome;;
-                (* buyer_call_timeout_action || seller_forfeit_dispute || seller_counter_dispute *)
-                backtrack[
-                    (1%nat, call purchase.(buyer) 0 (buyer_call_timeout purchaseId));
-                    (1%nat, call state.(seller) 0 (seller_forfeit_dispute purchaseId));
-                    (3%nat, call state.(seller) _item.(item_value) (seller_counter_dispute purchaseId random_bit))
-                ]
-          | counter =>
-                (* buyer_open_commitment || seller_call_timeout*)
-                backtrack[
-                    (1%nat, call purchase.(buyer) 0 (buyer_open_commitment purchaseId true 42%N));
-                    (4%nat, call state.(seller) 0 (seller_call_timeout purchaseId))
-
-                ]
-          | rejected | failed | completed => returnGen None
-          end
-      | _ => returnGen None
-      end);
-      (1% nat,
-               value <- bindGen (choose (1, 5)%Z) returnGenSome ;;  
-               call state.(seller) 0 (seller_update_listings itemId "updated description" value)
-      )
-      ]
-  | _, _ => returnGen None (* Should never happen *)
-  end.
-*)
 End EcommerceFixedGens.
