examples/ecommerce/tests/EcommerceGens.v
@@ -12,9 +12,8 @@ Import ListNotations.
 
 Module Type EcommerceGensInfo.
   Parameter contract_addr : Address.
-  Parameter purchase_buyer : Address.
-  Parameter item1_Id : nat.
-  Parameter purchaseId : N.
+  Parameter buyers : list Address.
+  Parameter item_ids : list nat.
 End EcommerceGensInfo.
 
 
@@ -25,6 +24,36 @@ Definition Env := Environment.
 Open Scope Z_scope.
 Local Open Scope string_scope.
     
+Definition constant_buyer_bit := true.
+Definition constant_buyer_nonce := 42%N.
+
+Definition is_active_purchase (key_purchase : (N * Purchase)) :=
+    let '(key, purchase) := key_purchase in
+    match purchase.(purchase_state) with
+    | completed | rejected | failed => false
+    | _ => true
+    end.
+
+Definition active_item_ids (state : State) :=
+    map fst (FMap.elements state.(listings)).
+
+(* Gets active buyer and a corresponding purchaseId *)
+Definition gActivePurchase (state : State) : GOpt (N * Purchase) :=
+    let actives_purchases := filter is_active_purchase (FMap.elements state.(purchases)) in
+    let address_purchaseId_purchases := map (fun '(key, purchase) => returnGenSome (key, purchase)) actives_purchases in
+    oneOf_ (returnGen None) address_purchaseId_purchases.
+
+Definition gOptRequestPurchase (state : State) : GOpt (Address * Amount * Msg) :=
+    buyer <- oneOf_ (returnGen None) (map returnGenSome buyers);;
+    itemId <- oneOf_ (returnGen None) (map returnGenSome (active_item_ids state));;
+    item <- returnGen (FMap.find itemId state.(listings));;
+    returnGenSome (buyer, item.(item_value), (buyer_request_purchase itemId "notes here")).
+
+Definition gOptUpdateListings (state : State) : GOpt (Address * Amount * Msg) :=
+    itemId <- bindGenOpt (oneOf_ (returnGen None) (map returnGenSome item_ids)) returnGenSome;;
+    value <- bindGen (choose (1,4)) returnGenSome;;
+    returnGenSome (state.(seller), 0, seller_update_listings itemId "updated description" value).
+    
 Definition gEcommerceAction (env : Env): GOpt Action :=
   let call caller amount msg :=
       returnGenSome {|
@@ -33,65 +62,60 @@ Definition gEcommerceAction (env : Env): GOpt Action :=
           act_body := act_call contract_addr amount (@serialize Ecommerce.Msg Ecommerce.Msg_serializable msg)
       |} in
   state <- returnGen (get_contract_state Ecommerce.State env contract_addr);;
-  let buyer_balance := env.(env_account_balances) purchase_buyer in
-  let itemId := item1_Id%nat in
-  let cur_slot := env.(env_chain).(current_slot) in
-  let buyer_dispute_delivery_commmitment := hash_bid purchaseId true 42%N in
-  match FMap.find itemId state.(listings), cur_slot with
-  | Some _item, 1%nat => (* This is done explicitly with cur_slot to make sure that we know the purchaseId in this generator. *)
-      (* buyer_request_purchase *)
-      call purchase_buyer _item.(item_value) (buyer_request_purchase itemId "notes here")
-  | Some _item, _ =>
   backtrack[
-    (19%nat,
-      match FMap.find purchaseId state.(purchases) with
-      | Some purchase => 
-          match purchase.(purchase_state) with
-          | requested =>
-                (* buyer_abort || seller_reject_contract || seller_accept_contract *)
-                backtrack [
-                    (1%nat, call purchase.(buyer) 0 (buyer_abort purchaseId));
-                    (1%nat, call state.(seller) 0 (seller_reject_contract purchaseId));
-                    (5%nat, call state.(seller) 0 (seller_accept_contract purchaseId))
-                ]
-          | accepted =>
-                (* buyer_call_timeout || seller_item_was_delivered *)
-                backtrack [
-                    (1%nat, call purchase.(buyer) 0 (buyer_call_timeout purchaseId));
-                    (4%nat, call state.(seller) 0 (seller_item_was_delivered purchaseId))
-                ]
-          | delivered =>
-                (* buyer_confirm_delivery || buyer_dispute_delivery || seller_call_timeout *)
-                backtrack [
-                    (1%nat, call purchase.(buyer) 0 (buyer_confirm_delivery purchaseId));
-                    (1%nat, call purchase.(buyer) 0 (buyer_dispute_delivery purchaseId buyer_dispute_delivery_commmitment));
-                    (4%nat, call state.(seller) 0 (seller_call_timeout purchaseId))
-                ]
-          | dispute =>
-                random_bit <- bindGen (oneOf[returnGen true; returnGen false]) returnGenSome;;
-                (* buyer_call_timeout_action || seller_forfeit_dispute || seller_counter_dispute *)
-                backtrack[
-                    (1%nat, call purchase.(buyer) 0 (buyer_call_timeout purchaseId));
-                    (1%nat, call state.(seller) 0 (seller_forfeit_dispute purchaseId));
-                    (3%nat, call state.(seller) 0 (seller_counter_dispute purchaseId random_bit))
-                ]
-          | counter =>
-                (* buyer_open_commitment || seller_call_timeout*)
-                backtrack[
-                    (1%nat, call purchase.(buyer) 0 (buyer_open_commitment purchaseId true 42%N));
-                    (4%nat, call state.(seller) 0 (seller_call_timeout purchaseId))
+    (* buyer_request_purchase *)
+    (4%nat, '(caller, amount, msg) <- gOptRequestPurchase state;;
+            call caller amount msg    
+    );
+    (* update_listings *)
+    (1%nat, '(caller, amount, msg) <- gOptUpdateListings state;;
+            call caller amount msg    
+    );
+    (** Purchase interactions **)
+    (15%nat,
+     '(purchaseId, purchase) <- gActivePurchase state;;
+     match purchase.(purchase_state) with
+        | requested =>
+            (* buyer_abort || seller_reject_contract || seller_accept_contract *)
+            backtrack [
+                (1%nat, call purchase.(buyer) 0 (buyer_abort purchaseId));
+                (1%nat, call state.(seller) 0 (seller_reject_contract purchaseId));
+                (5%nat, call state.(seller) 0 (seller_accept_contract purchaseId))
+            ]
+        | accepted =>
+            (* buyer_call_timeout || seller_item_was_delivered *)
+            backtrack [
+                (1%nat, call purchase.(buyer) 0 (buyer_call_timeout purchaseId));
+                (4%nat, call state.(seller) 0 (seller_item_was_delivered purchaseId))
+            ]
+        | delivered =>
+            (* buyer_confirm_delivery || buyer_dispute_delivery || seller_call_timeout *)
+            backtrack [
+                (1%nat, call purchase.(buyer) 0 (buyer_confirm_delivery purchaseId));
+                (1%nat, let buyer_dispute_delivery_commmitment := hash_bid purchaseId constant_buyer_bit constant_buyer_nonce in
+                        item <- returnGen (FMap.find purchase.(item) state.(listings));;
+                        call purchase.(buyer) item.(item_value) (buyer_dispute_delivery purchaseId buyer_dispute_delivery_commmitment));
+                (1%nat, call state.(seller) 0 (seller_call_timeout purchaseId))
+            ]
+        | dispute =>
+            (* buyer_call_timeout_action || seller_forfeit_dispute || seller_counter_dispute *)
+            backtrack[
+                (1%nat, call purchase.(buyer) 0 (buyer_call_timeout purchaseId));
+                (1%nat, call state.(seller) 0 (seller_forfeit_dispute purchaseId));
+                (3%nat, item <- returnGen (FMap.find purchase.(item) state.(listings));;
+                        random_bit <- bindGen (oneOf[returnGen true; returnGen false]) returnGenSome;;
+                        call state.(seller) item.(item_value) (seller_counter_dispute purchaseId random_bit))
+            ]
+        | counter =>
+            (* buyer_open_commitment || seller_call_timeout*)
+            backtrack[
+                (4%nat, call purchase.(buyer) 0 (buyer_open_commitment purchaseId constant_buyer_bit constant_buyer_nonce));
+                (1%nat, call state.(seller) 0 (seller_call_timeout purchaseId))
 
-                ]
-          | rejected | failed | completed => returnGen None
-          end
-      | _ => returnGen None
-      end);
-      (1% nat, (* Additional update listings here after a request to show error in property-based testing. *)
-               value <- bindGen (choose (1, 5)%Z) returnGenSome ;;  
-               call state.(seller) 0 (seller_update_listings itemId "updated description" value)
-      )
-      ]
-  | _, _ => returnGen None (* Should never happen *)
-  end.
-
+            ]
+        | rejected | failed | completed  => returnGen None (* should never happen! *)
+    end
+    )
+  ].
+  
 End EcommerceGens.
